Updates

generic/Zeta.GenericVerifier.fst
@@ -1,12 +1,76 @@
 module Zeta.GenericVerifier
 
-let get_record_set (#vspec: verifier_spec_base) (ss: S.seq (vspec.slot_t)) (vtls: vspec.vtls_t {vspec.valid vtls}):
-  (let record_t = app_record vspec.app.adm in
-   ors: option (S.seq record_t) {Some? ors ==> (let rs = Some?.v ors in
-                                                S.length rs = S.length ss /\
-                                                SA.distinct_elems ss /\
-                                                distinct_keys #vspec.app.adm rs)})
+let is_of_key (#adm) (ak: app_key adm) (r: app_record adm)
+  = fst r = ak
+
+open Zeta.SeqIdx
+
+let contains_key (#adm) (ak: app_key adm) (rs: S.seq (app_record adm))
+  = exists_elems_with_prop (is_of_key ak) rs
+
+let contains_key_comp (#adm) (ak: app_key adm) (rs: S.seq (app_record adm))
+  = exists_elems_with_prop_comp (is_of_key ak) rs
+
+let distinct_keys_snoc (#adm) (rs: S.seq (app_record adm)) (r: app_record adm)
+  : Lemma (ensures (let ak, av = r in
+                    distinct_keys rs ==>
+                    ~ (contains_key ak rs) ==>
+                    distinct_keys (SA.append1 rs r)))
+          [SMTPat (SA.append1 rs r)]
   = admit()
+
+let contains_app_key_base (#vspec: verifier_spec_base)
+  (vtls: vspec.vtls_t{ vspec.valid vtls })
+  (ss: S.seq (vspec.slot_t)) (i: SA.seq_index ss)
+  = let s = S.index ss i in
+    Some? (vspec.get s vtls) &&
+    (let gk,gv = Some?.v (vspec.get s vtls) in
+     Zeta.GenKey.AppK? gk)
+
+module IF = Zeta.IdxFnInt
+
+let gen_seq (#vspec: verifier_spec_base) (vtls: vspec.vtls_t {vspec.valid vtls}) =
+  {
+    IF.seq_t = S.seq vspec.slot_t;
+    IF.length = S.length;
+    IF.prefix = SA.prefix;
+  }
+
+let contains_app_key (#vspec: verifier_spec_base) (vtls: vspec.vtls_t {vspec.valid vtls})
+  : IF.idxfn_t (gen_seq vtls) bool
+  = contains_app_key_base vtls
+
+let to_app_record_base (#vspec: verifier_spec_base) (vtls: vspec.vtls_t {vspec.valid vtls})
+  (ss: S.seq vspec.slot_t) (i: SA.seq_index ss {contains_app_key vtls ss i})
+  = let s = S.index ss i in
+    let open Zeta.GenKey in
+    let AppK ak, AppV av = Some?.v (vspec.get s vtls) in
+    ak,av
+
+let to_app_record (#vspec: verifier_spec_base) (vtls: vspec.vtls_t {vspec.valid vtls})
+  : IF.cond_idxfn_t (app_record vspec.app.adm) (contains_app_key vtls)
+  = to_app_record_base vtls
+
+let get_record_set
+  (#vspec: verifier_spec_base)
+  (ss: S.seq (vspec.slot_t))
+  (vtls: vspec.vtls_t {vspec.valid vtls})
+  : Tot (let record_t = app_record vspec.app.adm in
+         ors: option (S.seq record_t) {Some? ors ==> (let rs = Some?.v ors in
+                                       S.length rs = S.length ss /\
+                                       SA.distinct_elems ss /\
+                                       distinct_keys #vspec.app.adm rs)})
+  = let open FStar.Seq in
+    let open Zeta.SeqAux in
+    let open Zeta.AppSimulate.Helper in
+    let fm = IF.to_fm (contains_app_key vtls) (to_app_record vtls) in
+    let rs = IF.filter_map fm ss in
+    if distinct_elems_comp ss && S.length rs = S.length ss && distinct_keys_comp rs then
+      Some rs
+    else None
+
+
+#push-options "--fuel 0 --ifuel 1 --query_stats"
 
 let get_record_set_correct
   (#vspec: _)
@@ -22,8 +86,15 @@ let get_record_set_correct
                      let open Zeta.GenKey in
                      gk = AppK ak /\
                      gv = AppV av)))
-  = admit()
+  = let open FStar.Seq in
+    let open Zeta.SeqAux in
+    let open Zeta.AppSimulate.Helper in
+    let fm = IF.to_fm (contains_app_key vtls) (to_app_record vtls) in
+    let rs = IF.filter_map fm ss in
+    assert(distinct_elems ss /\ S.length rs = S.length ss /\ distinct_keys rs);
+    IF.lemma_idx2fidx_idem (contains_app_key vtls) ss i
 
+#pop-options
 
 let update_record_set (#vspec: verifier_spec_base)
                       (ss: S.seq (vspec.slot_t))
